AVL_incorrect.v
@@ -1,0 +1,1478 @@
+Require Import ssreflect Utf8 CpdtTactics Util FunInd.
+Require Import Arith Orders OrdersTac OrdersFacts.
+Require Import DecidableClass.
+Require Import ssrbool.
+Require Import FrapWithoutSets.
+Require Import Psatz.
+From Coq.micromega Require Import RingMicromega QMicromega EnvRing Tauto Zify.
+Require Import Classical ClassicalDescription IndefiniteDescription.
+
+Set Implicit Arguments.
+Close Scope string_scope.
+Close Scope boolean_if_scope.
+Open Scope general_if_scope.
+Close Scope Z_scope.
+
+
+(* we're going to say no to setoid hell today, please give us the usual equality thank you *)
+Module AVL (OT : UsualOrderedType').
+  Include EqLtNotation OT.
+  Include CmpNotation OT OT.
+
+  Include OrderedTypeFacts OT.
+  Include OrderedTypeTest OT.
+
+  Local Notation A := OT.t.
+  Notation compare := OT.compare.
+
+  Local Notation Eq := Datatypes.Eq.
+  Local Notation Lt := Datatypes.Lt.
+  Local Notation Gt := Datatypes.Gt.
+
+  Hint Rewrite compare_eq_iff compare_lt_iff compare_gt_iff : core.
+  Hint Extern 1 => order : core.
+  (* Hint Rewrite compare_refl : core. *)
+
+  (* if we're trying to match a compare in the goal,
+  then we automatically simplify it depending on the assumptions present.  *)
+  Ltac rewrite_match_compare :=
+    match goal with
+    | [ |- context[match compare ?x ?x with | _ => _ end] ] =>
+        rewrite compare_refl
+    | [ H : ?x < ?y |- context[match compare ?x ?y with | _ => _ end] ] =>
+        rewrite (proj2 (compare_lt_iff x y) H)
+    | [ H : ?y < ?x |- context[match compare ?x ?y with | _ => _ end] ] =>
+        rewrite (proj2 (compare_gt_iff x y) H)
+    end.
+  Hint Extern 1 => rewrite_match_compare : core.
+
+  Ltac case_compare' x y :=
+    let i := fresh "Heq" in
+    let e := fresh in
+    remember (compare x y) as e eqn:i;
+    symmetry in i;
+    destruct e; simplify; try order.
+  (* A variant that also adds `crush` to try to close out as many goals as possible. *)
+  Ltac case_compare x y :=
+    case_compare' x y; crush; try order.
+
+  (* binary tree of our ordered type *)
+  Inductive tree : Type :=
+  | Nil  : tree
+  | Node : ∀ (v : A) (l : tree) (r : tree), tree.
+  Hint Constructors tree : core.
+  (* in this file, we don't bother with storing the heights or sizes as in-node information.
+  * as a consequence, all operations are far slower than they actually could be.
+  * the trade-off is that we have less to juggle. *)
+
+  Definition singleton x : tree := Node x Nil Nil.
+
+  (* get the height of a tree  *)
+  Fixpoint height (t : tree) : nat :=
+    match t with
+    | Nil => 0
+    | Node _ l r => 1 + Nat.max (height l) (height r)
+    end.
+
+  Fixpoint size (t : tree) : nat :=
+    match t with
+    | Nil => 0
+    | Node _ l r => 1 + (size l) + (size r)
+    end.
+
+  Section Contains_In.
+
+    (* returns true if x in t else false; only guaranteed if t is a BST *)
+    Fixpoint Containsb x t : bool :=
+      match t with
+      | Nil => false
+      | Node v l r =>
+          match (v ?= x) with
+          | Eq => true
+          | Gt => Containsb x l
+          | Lt => Containsb x r
+          end
+      end.
+    Locate Eq.
+
+    (* prop-valued version *)
+    Fixpoint Contains x t : Prop :=
+      match t with
+      | Nil => False
+      | Node v l r =>
+          match (v ?= x) with
+          | Eq => True
+          | Gt => Contains x l
+          | Lt => Contains x r
+          end
+      end.
+
+    (* And as an inductive proposition instead *)
+    Inductive Contains' (x : A) : tree → Prop :=
+    | Contains'_node  : ∀ l r,   Contains' x (Node x l r)
+    | Contains'_left  : ∀ y l r, Contains' x l → x < y → Contains' x (Node y l r)
+    | Contains'_right : ∀ y l r, Contains' x r → y < x → Contains' x (Node y l r).
+    Hint Constructors Contains' : core.
+
+    Lemma Contains_Nil_False x : ¬ Contains x Nil.
+    Proof.
+      by crush.
+    Qed.
+
+    Lemma Contains'_Nil_False x : ¬ Contains' x Nil.
+    Proof.
+      move=> H; by invert H.
+    Qed.
+
+    Lemma Contains_not_Nil x t : Contains x t → t ≠ Nil.
+    Proof.
+      by crush.
+    Qed.
+
+    Lemma Contains'_not_Nil x t : Contains' x t → t ≠ Nil.
+    Proof.
+      move=> H bad; by invert H.
+    Qed.
+
+    (* These two definitions capture the same notion. *)
+    Lemma Contains'_iff_Contains x t : Contains' x t ↔ Contains x t.
+    Proof.
+      split; induction t.
+      - move=> H; by invert H.
+      - move=> H; invert H; by crush.
+      - move=> H; by crush.
+      - move=> H; crush; by case_compare v x.
+      (* this case_compare actually invokes rewrite_match_compare! *)
+    Qed.
+
+    Hint Resolve
+      Contains_Nil_False Contains'_Nil_False
+      Contains_not_Nil Contains'_not_Nil : core.
+
+    Hint Rewrite Contains'_iff_Contains : core.
+
+    (* a true "Contains" which works on any tree, not just BST *)
+    Fixpoint In (x : A) (t : tree) : Prop :=
+      match t with
+      | Nil => False
+      | Node v l r =>
+          v = x ∨ In x l ∨ In x r
+      end.
+
+    (* As an inductive proposition instead. *)
+    Inductive In'  (x : A) : tree → Prop :=
+    | In'_node      : ∀ l r, In' x (Node x l r)
+    | In'_left      : ∀ y l r, In' x l → In' x (Node y l r)
+    | In'_right     : ∀ y l r, In' x r → In' x (Node y l r).
+    Hint Constructors In' : core.
+    Arguments In'_node [x] l r.
+
+    Lemma In_Nil_False x : ¬ In x Nil.
+    Proof.
+      by crush.
+    Qed.
+
+    Lemma In_not_Nil x t : In x t → t ≠ Nil.
+    Proof.
+      by crush.
+    Qed.
+
+    Lemma In'_Nil_False x : ¬ In' x Nil.
+    Proof.
+      move=> H; by invert H.
+    Qed.
+
+    Lemma In'_not_Nil x t : In' x t → t ≠ Nil.
+    Proof.
+      move=> H bad; by invert H.
+    Qed.
+
+    Hint Resolve In_Nil_False In_not_Nil In'_Nil_False In'_not_Nil : core.
+
+    (* These two definitions capture the exact same thing. *)
+    Lemma In'_iff_In x t : In' x t ↔ In x t.
+    Proof.
+      split; induction t.
+      - move=> H; by invert H.
+      - move=> H.
+        invert H; by crush.
+      - move=> H; by invert H.
+      - rewrite /In.
+        by case_compare v x.
+    Qed.
+    Hint Rewrite In'_iff_In : core.
+
+    (* `Contains` is a strictly stronger condition than In. *)
+    Lemma Contains_In x t : Contains x t → In x t.
+    Proof.
+      induction t.
+      - done.
+      - rewrite /Contains /In; move=> Contains_x.
+        by case_compare v x.
+    Qed.
+    Hint Resolve Contains_In : core.
+
+  End Contains_In.
+  Hint Constructors In' Contains' : core.
+  Hint Resolve
+    Contains_Nil_False Contains'_Nil_False
+    Contains_not_Nil Contains'_not_Nil
+    In_Nil_False In_not_Nil In'_Nil_False In'_not_Nil
+    Contains_In
+    : core.
+  Hint Rewrite Contains'_iff_Contains : core.
+
+  (* a really simple tactic to deconstruct ands/ors of bools *)
+  Ltac simplify_bool :=
+    repeat match goal with
+    | [H: (?a && ?b) = true |- _ ] =>
+        let H1 := fresh in
+        let H2 := fresh in
+        have {H}[H1 H2] := andb_prop _ _ H
+    | [H: (?a || ?b) = false |- _] =>
+        let H1 := fresh in
+        let H2 := fresh in
+        have {H}[H1 H2] := orb_false_elim _ _ H
+    | [H: (?a || ?b) = true |- _] =>
+        apply orb_prop in H;
+        invert H
+    | [H: (?a && ?b) = false |- _] =>
+        apply andb_false_elim in H;
+        invert H
+    end.
+  Hint Extern 2 => simplify_bool : core.
+
+  Section AnyAll.
+
+    Fixpoint Any (P : A → Prop) (t : tree) : Prop :=
+      match t with
+      | Nil => False
+      | Node v l r =>
+          P v ∨ Any P l ∨ Any P r
+      end.
+
+    Fixpoint Anyb (P : A → bool) (t : tree) : bool :=
+      match t with
+      | Nil => false
+      | Node v l r =>
+          P v || Anyb P l || Anyb P r
+      end.
+
+    Fixpoint All (P : A → Prop) (t : tree) : Prop :=
+      match t with
+      | Nil => True
+      | Node v l r =>
+          P v ∧ All P l ∧ All P r
+      end.
+
+    Fixpoint Allb (P : A → bool) (t : tree) : bool :=
+      match t with
+      | Nil => true
+      | Node v l r =>
+          P v && Allb P l && Allb P r
+      end.
+
+    Lemma Any_Nil_False P : ¬ Any P Nil.
+    Proof.
+      by crush.
+    Qed.
+
+    (* Note here: for both of these iff results, we use In' rather than In,
+     * since chances are, if you actually need to rewrite away from the fixpoint Any
+     * to prove something, you probably want to have an inductive In'
+     * (which you can then perform case analysis on) instead of a fixpoint In.
+     *)
+    Lemma Any_iff_exists P t :
+      Any P t ↔ (∃ x, In' x t ∧ P x).
+    Proof.
+      split.
+      - (* forwards *)
+        setoid_rewrite In'_iff_In.
+        induction t.
+        + by crush.
+        + move => [H|[H|H]].
+          * exists v; by crush.
+          * have {H}[x [x_In' Px]] := IHt1 H.
+            exists x; by crush.
+          * have {H}[x [x_In' Px]] := IHt2 H.
+            exists x; by crush.
+      - (* backwards *)
+        move=> [x [x_In' Px]].
+        induction x_In'; by crush.
+    Qed.
+
+    Lemma All_iff_forall P t :
+      All P t ↔ (∀ x, In' x t → P x).
+    Proof.
+      split.
+      - (* forwards *)
+        setoid_rewrite In'_iff_In.
+        induction t; by crush.
+      - (* backwards *)
+        move=> H.
+        induction t; by crush.
+    Qed.
+
+    (* Hint Rewrite Any_iff_exists All_iff_forall : core. *)
+
+
+    Lemma Allb_iff_All P t : Allb P t = true ↔ All (fun x => P x = true) t.
+    Proof.
+      induction t; by crush.
+    Qed.
+
+    Lemma Anyb_iff_Any P t : Anyb P t = true ↔ Any (fun x => P x = true) t.
+    Proof.
+       induction t; by crush.
+    Qed.
+
+    (* we can weaken on All *)
+    Lemma All_imp (p : A → Prop) {q : A → Prop} (H : ∀ {x}, p x → q x) :
+      ∀ {t}, All p t → All q t.
+    Proof.
+      induction t; by crush.
+    Qed.
+
+    Lemma Allb_spec0 P t : reflect (All (fun x => P x = true) t) (Allb P t).
+    Proof.
+      move Heq : (Allb P t) => b.
+      destruct b.
+      - setoid_rewrite Allb_iff_All in Heq.
+        by constructor.
+      - constructor.
+        setoid_rewrite <-Allb_iff_All.
+        by crush.
+    Defined.
+
+    Lemma All_dec (P : A → Prop) (t : tree) :
+      (∀ x, {P x} + {¬ P x}) → {All P t} + {¬ All P t}.
+    Proof.
+      move=>P_dec.
+      induction t.
+      - by left.
+      - destruct (P_dec v) as [Px|Px], IHt1 as [IHt1|IHt1], IHt2 as [IHt2|IHt2].
+        all: try (right; by crush).
+        by left.
+    Defined.
+
+    Lemma Any_dec (P : A → Prop) (t : tree) :
+      (∀ x, {P x} + {¬ P x}) → {Any P t} + {¬ Any P t}.
+    Proof.
+      move=>P_dec.
+      induction t.
+      - by right.
+      - destruct (P_dec v) as [Px|Px], IHt1 as [IHt1|IHt1], IHt2 as [IHt2|IHt2].
+        all: try (left; by crush).
+        right; by crush.
+    Defined.
+
+  End AnyAll.
+  Hint Resolve All_dec Any_dec : core.
+  Hint Rewrite Allb_iff_All Anyb_iff_Any Any_iff_exists : core.
+  (* Hint Rewrite All_iff_forall Any_iff_exists Allb_iff_All Anyb_iff_Any : core. *)
+
+  Section Rotations.
+    (* rotate root towards left *)
+    Definition rotate_left v l r : tree :=
+      match r with
+      | Node rv rl rr => Node rv (Node v l rl) rr
+      | r => Node v l r
+      end.
+
+    (* rotate root towards right *)
+    Definition rotate_right (v : A) (l r : tree) : tree :=
+      match l with
+      | Node lv ll lr => Node lv ll (Node v lr r)
+      | l => Node v l r
+      end.
+
+    (* left heavy *)
+    Definition balance_left (v : A) (l r : tree) : tree :=
+      if (1 + height r) <? (height l) then
+        match l with
+        (* this is never true in a well-formed AVL tree *)
+        | Nil => Node v l r
+        (* rather, we will always be in this case *)
+        | Node lv ll lr as l =>
+            if height lr <? height ll then
+              (* left-left, one rotation *)
+              rotate_right v l r
+            else
+              (* left-right, two rotations *)
+              rotate_right v (rotate_left lv ll lr) r
+        end
+      else
+        Node v l r.
+
+    (* right heavy *)
+    Definition balance_right (v : A) (l r : tree) : tree :=
+      if 1 + height l <? height r then
+        match r with
+        | Nil => Node v l r
+        | Node rv rl rr as r =>
+            if height rl <? height rr then
+              (* right-right, one rotation *)
+              rotate_left v l r
+            else
+              (* right-left, two rotations *)
+              rotate_left v l (rotate_right rv rl rr)
+        end
+      else
+        Node v l r.
+
+  End Rotations.
+  Functional Scheme rotate_left_ind := Induction for rotate_left Sort Prop.
+  Functional Scheme rotate_right_ind := Induction for rotate_right Sort Prop.
+  Functional Scheme balance_left_ind := Induction for balance_left Sort Prop.
+  Functional Scheme balance_right_ind := Induction for balance_right Sort Prop.
+
+  Section InsertDelete.
+
+  Fixpoint insert x t :=
+    match t with
+    | Nil => Node x Nil Nil
+    | Node v l r =>
+        match (v ?= x) with
+        | Eq => Node v l r
+        | Lt => balance_right v l (insert x r)
+        | Gt => balance_left  v (insert x l) r
+        end
+    end.
+
+  Fixpoint stupid_insert x t :=
+    match t with
+    | Nil => Node x Nil Nil
+    | Node v l r =>
+        match (v ?= x) with
+        | Eq => Node v l r
+        | Lt => Node v l (stupid_insert x r)
+        | Gt => Node v (stupid_insert x l) r
+        end
+    end.
+
+  (* shrink_max removes and returns the maximum (right-most) element of a tree *)
+  Fixpoint shrink_max (t : tree) : option A * tree :=
+    match t with
+    | Nil => (None, Nil)
+    | Node v l r =>
+        match shrink_max r with
+        | (None, _) => (Some v, l)
+        | (Some x, r') => (Some x, balance_right v l r')
+        end
+    end.
+
+  (* del_root l r deletes the root, t = (Node _ l r).
+  * it accomplishes this by swapping the root node's value with the max element of its left subtree,
+  * then deleting the max element instead.
+  *)
+  Definition del_root (l r : tree) : tree :=
+    match shrink_max l with
+    | (None, _) => r
+    | (Some x, l') => balance_right x l' r
+    end.
+
+  Fixpoint delete x t :=
+    match t with
+    | Nil => Nil
+    | Node v l r =>
+        match (v ?= x) with
+        | Eq => del_root l r
+        | Lt => balance_left  v l (delete x r)
+        | Gt => balance_right v (delete x l) r
+        end
+    end.
+
+  Inductive path : Type :=
+  | Path_root  : path
+  | Path_left  : ∀ (parent : path) (v : A) (r : tree), path
+  | Path_right : ∀ (parent : path) (v : A) (l : tree), path.
+
+  Fixpoint get_path' x t p : tree * path :=
+    match t with
+    | Nil => (Nil, p)
+    | Node v l r =>
+        match (v ?= x) with
+        | Eq => (Node v l r, p)
+        | Lt => get_path' x r (Path_right p v l)
+        | Gt => get_path' x l (Path_left  p v r)
+        end
+    end.
+  Definition get_path x t : tree * path := get_path' x t Path_root.
+  End InsertDelete.
+  Functional Scheme insert_ind := Induction for insert Sort Prop.
+  Functional Scheme del_root_ind := Induction for del_root Sort Prop.
+  Functional Scheme shrink_max_ind := Induction for shrink_max Sort Prop.
+  Functional Scheme delete_ind := Induction for delete Sort Prop.
+  Hint Constructors path : core.
+
+  Section OfToList.
+    Definition of_list (l : list A) : tree :=
+      fold_right insert Nil l.
+
+    Fixpoint to_list (t : tree) : list A :=
+      match t with
+      | Nil => []
+      | Node v l r => (to_list l) ++ v :: (to_list r)
+      end.
+  End OfToList.
+
+  Section WF_def.
+    (* is our tree actually a BST? *)
+    Fixpoint Ordered (t : tree) : Prop :=
+      match t with
+      | Nil => True
+      | Node v l r =>
+          (All (fun x => x < v) l ∧ Ordered l) ∧ (All (fun x => v < x) r ∧ Ordered r)
+      end.
+
+    Inductive Ordered' : tree → Prop :=
+    | Ordered'_nil  : Ordered' Nil
+    | Ordered'_node :
+      ∀ v l r, All (fun x => x < v) l → Ordered' l →
+               All (fun x => v < x) r → Ordered' r →
+               Ordered' (Node v l r).
+    Hint Constructors Ordered' : core.
+
+    (* does the AVL invariant hold? *)
+    Inductive Balanced : tree → Prop :=
+    (* a leaf node is Balanced *)
+    | Balanced_nil : Balanced Nil
+    (* two children of equal height is Balanced *)
+    | Balanced_equal :
+      ∀ l r, Balanced l → Balanced r → height l = height r → ∀ v, Balanced (Node v l r)
+    (* if height l = height r + 1, then the resulting thing is Balanced *)
+    | Balanced_left_heavy :
+      ∀ l r, Balanced l → Balanced r → height l = 1 + height r → ∀ v, Balanced (Node v l r)
+    (* symmetric. *)
+    | Balanced_right_heavy :
+      ∀ l r, Balanced l → Balanced r → 1 + height l = height r → ∀ v, Balanced (Node v l r).
+    Hint Constructors Balanced : core.
+
+    (* well-formedness invariant *)
+    Inductive WF : tree → Prop :=
+    (* an AVL tree (that is, a well-formed tree) is ordered and has the balance invariant *)
+    | WF_base :
+      ∀ t, Ordered t → Balanced t → WF t
+    (* inserting into a well-formed tree results in a well-formed tree *)
+    | WF_insert :
+      ∀ t, WF t → ∀ x, WF (insert x t)
+    (* deleting from a well-formed tree results in a well-formed tree *)
+    | WF_delete :
+      ∀ t, WF t → ∀ x, WF (delete x t).
+    Hint Constructors WF : core.
+
+
+  End WF_def.
+  Hint Constructors Ordered' Balanced WF : core.
+
+  Ltac invert_ordered' :=
+    repeat match goal with
+    | [ H : Ordered' (Node _ _ _) |- _ ] => invert H
+    end.
+
+  Tactic Notation "split_ifs" ident(h) :=
+    match goal with
+    | [ |- context[if ?exp then _ else _ ] ] =>
+        let i := fresh h in
+        let b := fresh in
+        move i : exp => b;
+        destruct b
+    end.
+  Tactic Notation "split_ifs" := split_ifs Hb.
+
+  Ltac ltb_to_lt :=
+    match goal with
+    | [ H : (?a <? ?b)%nat = true |- _ ] => rewrite Nat.ltb_lt in H
+    | [ H : (?a <? ?b)%nat = false |- _ ] => rewrite Nat.ltb_ge in H
+    end.
+  Hint Rewrite Nat.ltb_lt Nat.ltb_ge : core.
+
+  Ltac match_compare :=
+    rewrite_match_compare ||
+    match goal with
+    | [ |- context[match compare ?v ?x with |_ => _ end] ] =>
+        elim_compare v x
+    end.
+  Hint Extern 1 => match_compare : core.
+
+  Hint Rewrite Nat.max_id : core.
+
+
+  Lemma height_eq_zero_nil t : height t = 0 → t = Nil.
+  Proof.
+    by destruct t.
+  Qed.
+
+  Lemma height_eq_one_singleton t : height t = 1 → ∃ v, t = Node v Nil Nil.
+  Proof.
+    move => t_height.
+    destruct t.
+    - by crush.
+    - exists v.
+      invert t_height.
+      have t1_zero : (height t1) = 0 by lia.
+      have t2_zero : (height t2) = 0 by lia.
+      by rewrite (height_eq_zero_nil _ t1_zero) (height_eq_zero_nil _ t2_zero).
+  Qed.
+
+  Lemma size_eq_zero_nil t : size t = 0 → t = Nil.
+  Proof.
+    by destruct t.
+  Qed.
+
+  Lemma size_eq_one_singleton t : size t = 1 → ∃ v, t = Node v Nil Nil.
+  Proof.
+    move => t_size.
+    destruct t.
+    - by crush.
+    - exists v.
+      invert t_size.
+      have t1_zero : size t1 = 0 by lia.
+      have t2_zero : size t2 = 0 by lia.
+      by rewrite (size_eq_zero_nil _ t1_zero) (size_eq_zero_nil _ t2_zero).
+  Qed.
+
+  Lemma node_neq_nil {v l r} : Node v l r ≠ Nil.
+    by crush.
+  Qed.
+
+  Lemma nil_neq_node {v l r} : Nil ≠ Node v l r.
+    by crush.
+  Qed.
+
+  Hint Resolve node_neq_nil nil_neq_node : core.
+
+  (* Section Facts. *)
+
+    Lemma All_lt_dec v l : {All (fun x => x < v) l} + {¬ All (fun x => x < v) l}.
+    Proof.
+      apply All_dec.
+      move=>x.
+      by apply lt_dec.
+    Defined.
+
+    Lemma All_gt_dec v r : {All (fun x => v < x) r} + {¬ All (fun x => v < x) r}.
+    Proof.
+      apply All_dec.
+      move=>x; by apply lt_dec.
+    Defined.
+
+    Lemma Ordered_dec t : {Ordered t} + {¬ Ordered t}.
+    Proof.
+      induction t.
+      - by left.
+      - destruct IHt1, IHt2, (All_lt_dec v t1), (All_gt_dec v t2).
+        all: try (right; by crush).
+        left; by crush.
+    Defined.
+
+    Lemma Ordered_iff_Ordered' t : Ordered t ↔ Ordered' t.
+    Proof.
+      split.
+      - move=>Ordered_t .
+        induction t.
+        + by constructor.
+        + crush; by constructor.
+      - move=>Ordered_t.
+        induction Ordered_t; by crush.
+    Qed.
+    Hint Rewrite Ordered_iff_Ordered' : core.
+
+    (* Contains behaves exactly like In when the tree is Ordered. *)
+    Lemma Ordered_In_Contains x t : Ordered t → In x t → Contains x t.
+    Proof.
+      move=>t_Ordered x_In.
+      rewrite -In'_iff_In in x_In.
+      induction x_In.
+      - by crush.
+      - crush.
+        rewrite All_iff_forall in H1.
+        specialize (H1 x x_In).
+        by match_compare.
+        (* rewrite All_iff_forall in H1. *)
+        (* specialize (H1 x x_In). *)
+        (* by case_compare y x. *)
+      - crush.
+        rewrite All_iff_forall in H.
+        specialize (H x x_In).
+        by match_compare.
+    Qed.
+
+    Lemma Ordered_In_iff_Contains x t : Ordered t → In x t ↔ Contains x t.
+    Proof.
+      move=>t_Ordered.
+      split.
+      - by apply: Ordered_In_Contains.
+      - by apply: Contains_In.
+    Qed.
+
+    Lemma rotate_left_preserves_Ordered v l r : Ordered (Node v l r) → Ordered (rotate_left v l r).
+    Proof.
+      rewrite !Ordered_iff_Ordered' /rotate_left.
+      move=>ordered.
+      destruct r; invert_ordered'; try by constructor.
+      constructor; crush.
+      apply (All_imp (fun x => x < v)); crush.
+      (* - apply (All_imp (fun x => x < v)); crush. *)
+      (* - constructor; by crush. *)
+    Qed.
+
+    Lemma rotate_right_preserves_Ordered v l r : Ordered (Node v l r) → Ordered (rotate_right v l r).
+    Proof.
+      rewrite !Ordered_iff_Ordered' /rotate_right.
+      intros; destruct l; invert_ordered'; try by constructor.
+      constructor; crush.
+      apply (All_imp (fun x => v < x)); by crush.
+      (* - apply (All_imp (fun x => v < x)); by crush. *)
+      (* - constructor; by crush. *)
+    Qed.
+
+    Lemma rotate_left_preserves_Ordered' v l r : Ordered' (Node v l r) → Ordered' (rotate_left v l r).
+      rewrite -!Ordered_iff_Ordered'.
+      exact: rotate_left_preserves_Ordered.
+    Qed.
+
+    Lemma rotate_right_preserves_Ordered' v l r : Ordered' (Node v l r) → Ordered' (rotate_right v l r).
+      rewrite -!Ordered_iff_Ordered'.
+      exact: rotate_right_preserves_Ordered.
+    Qed.
+
+
+    (* Tactic Notation "split_ifs" := let h := fresh in split_ifs h. *)
+      (* repeat match goal with *)
+      (* | [ |- context[if ?b then _ else _ ] ] => *)
+      (*     let i := fresh "Heq" in *)
+      (*     let e := fresh in *)
+      (*     move i : b => e; *)
+      (*     destruct e *)
+      (* end. *)
+
+    Lemma rotate_left_preserves_All P v l r : (All P (Node v l r)) → All P (rotate_left v l r).
+    Proof.
+      move=>[Pv [Pl Pr]].
+      destruct r; by crush.
+    Qed.
+
+    Lemma rotate_right_preserves_All P v l r : All P (Node v l r) → All P (rotate_right v l r).
+    Proof.
+      destruct l; by crush.
+    Qed.
+
+    Ltac unrotate :=
+      match goal with
+      | [ |- All _ (rotate_left _ _ _) ] => eapply rotate_left_preserves_All
+      | [ |- All _ (rotate_right _ _ _) ] => eapply rotate_right_preserves_All
+      | [ |- Ordered' (rotate_left _ _ _) ] => eapply rotate_left_preserves_Ordered'
+      | [ |- Ordered' (rotate_right _ _ _) ] => eapply rotate_right_preserves_Ordered'
+      end.
+    Hint Extern 1 => unrotate : core.
+
+    (* Hint Resolve rotate_left_preserves_Ordered' rotate_right_preserves_Ordered' : core. *)
+    (* Hint Resolve rotate_left_preserves_All rotate_right_preserves_All : core. *)
+
+    Lemma balance_left_preserves_Ordered v l r : Ordered (Node v l r) → Ordered (balance_left v l r).
+    Proof.
+      move => H_order.
+      have := H_order.
+      rewrite !Ordered_iff_Ordered' /balance_left.
+      intros; invert_ordered'.
+      split_ifs.
+      - destruct l.
+        + by crush.
+        + crush.
+          split_ifs.
+          * constructor; crush.
+            apply (All_imp (fun x => v < x)); by crush.
+            (* -- apply (All_imp (fun x => v < x)); by crush. *)
+            (* -- constructor; by crush. *)
+          * unrotate.
+            constructor; crush.
+            unrotate; by crush.
+      - destruct l.
+        + constructor; by crush.
+        + try repeat constructor; by crush.
+    Qed.
+
+    Lemma balance_right_preserves_Ordered v l r : Ordered (Node v l r) → Ordered (balance_right v l r).
+    Proof.
+      move => H_order.
+      have := H_order.
+      rewrite !Ordered_iff_Ordered' /balance_right.
+      intros; invert_ordered'.
+      split_ifs.
+      - destruct r; try repeat constructor; crush.
+        split_ifs; try repeat constructor; crush.
+        + apply (All_imp (fun x => x < v)); by crush.
+        + unrotate; repeat constructor; crush.
+          unrotate; by crush.
+      - destruct r; try repeat constructor; by crush.
+    Qed.
+
+    Lemma balance_left_preserves_Ordered' v l r : Ordered' (Node v l r) → Ordered' (balance_left v l r).
+    Proof.
+      rewrite -!Ordered_iff_Ordered'.
+      exact: balance_left_preserves_Ordered.
+    Qed.
+
+    Lemma balance_right_preserves_Ordered' v l r : Ordered' (Node v l r) → Ordered' (balance_right v l r).
+    Proof.
+      rewrite -!Ordered_iff_Ordered'.
+      exact: balance_right_preserves_Ordered.
+    Qed.
+
+    (* Hint Resolve balance_left_preserves_Ordered : core. *)
+    Lemma balance_left_preserves_All P v l r : All P (Node v l r) → All P (balance_left v l r).
+    Proof.
+      move=> Pt.
+      rewrite /balance_left.
+      split_ifs; destruct l; try repeat (split_ifs || constructor || unrotate); crush; done.
+    Qed.
+
+    Lemma balance_right_preserves_All P v l r : All P (Node v l r) → All P (balance_right v l r).
+    Proof.
+      move=> Pt.
+      rewrite /balance_right.
+      split_ifs; destruct r; try repeat (split_ifs || constructor || unrotate); crush; done.
+    Qed.
+
+    Lemma insert_preserves_All P x t : All P t → P x → All P (insert x t).
+    Proof.
+      move=>Pt Px.
+      induction t.
+      - by crush.
+      - crush.
+        match_compare; crush;
+          (apply balance_left_preserves_All || apply balance_right_preserves_All); crush;
+          done.
+    Qed.
+
+    Lemma insert_preserves_Ordered' x t : Ordered' t → Ordered' (insert x t).
+    Proof.
+      move=>t_Ordered.
+      induction t_Ordered; crush.
+      - repeat constructor; by crush.
+      - match_compare; repeat constructor; crush;
+        (apply balance_left_preserves_Ordered' || apply balance_right_preserves_Ordered');
+        repeat constructor; crush;
+        apply insert_preserves_All; crush;
+        done.
+    Qed.
+
+    Lemma In_singleton x y : In y (Node x Nil Nil) → y = x.
+    Proof.
+      crush.
+    Qed.
+
+    Lemma rotate_left_In_complete x v l r : In x (Node v l r) → In x (rotate_left v l r).
+    Proof.
+      move => H_In.
+      destruct r; simpl;
+      by repeat match goal with
+      | [ H : In _ (Node _ _ _) |- _ ] => destruct H; subst; eauto
+      | [ H : _ ∨ _ |- _] => destruct H; subst; eauto
+      end.
+    Qed.
+
+    Lemma rotate_right_In_complete x v l r : In x (Node v l r) → In x (rotate_right v l r).
+    Proof.
+      move => H_In.
+      destruct l; simpl;
+      by repeat match goal with
+      | [ H : In _ (Node _ _ _) |- _ ] => destruct H; subst; eauto
+      | [ H : _ ∨ _ |- _] => destruct H; subst; eauto
+      end.
+    Qed.
+
+    Lemma rotate_left_In_correct x v l r : In x (rotate_left v l r) → In x (Node v l r).
+    Proof.
+      destruct r; simpl; tauto.
+    Qed.
+
+    Lemma rotate_right_In_correct x v l r : In x (rotate_right v l r) → In x (Node v l r).
+    Proof.
+      destruct l; simpl; tauto.
+    Qed.
+
+    Lemma rotate_left_In_iff x v l r : In x (rotate_left v l r) <-> In x (Node v l r).
+    Proof.
+      split; by eauto using rotate_left_In_correct, rotate_left_In_complete.
+    Qed.
+
+    Lemma rotate_right_In_iff x v l r : In x (rotate_right v l r) <-> In x (Node v l r).
+      split; by eauto using rotate_right_In_correct, rotate_right_In_complete.
+    Qed.
+
+    Hint Extern 1 (In _ (rotate_left _ _ _)) => eapply rotate_left_In_complete : core.
+    Hint Extern 1 (In _ (rotate_right _ _ _)) => eapply rotate_right_In_complete : core.
+    Hint Rewrite rotate_left_In_iff rotate_right_In_iff : core.
+
+    Lemma rotate_left_In_tac1 x v lv ll lr r : In x (Node v (Node lv ll lr) r) → In x (Node v (rotate_left lv ll lr) r).
+    Proof.
+      move => H.
+      destruct H as [H | [ H | H ]]; subst.
+      all: try by (rewrite /In; propositional).
+      right; left; by rewrite rotate_left_In_iff.
+    Qed.
+
+    Lemma rotate_left_In_tac2 x v l rv rl rr : In x (Node v l (Node rv rl rr)) → In x (Node v l (rotate_left rv rl rr)).
+    Proof.
+      move => H.
+      destruct H as [H | [H | H]]; subst; try by (rewrite /In; propositional).
+      right; right; by rewrite rotate_left_In_iff.
+    Qed.
+
+    Lemma rotate_right_In_tac1 x v lv ll lr r : In x (Node v (Node lv ll lr) r) → In x (Node v (rotate_right lv ll lr) r).
+    Proof.
+      move => H.
+      destruct H as [H | [ H | H ]]; subst.
+      all: try by (rewrite /In; propositional).
+      right; left; by rewrite rotate_right_In_iff.
+    Qed.
+
+    Lemma rotate_right_In_tac2 x v l rv rl rr : In x (Node v l (Node rv rl rr)) → In x (Node v l (rotate_right rv rl rr)).
+    Proof.
+      move => H.
+      destruct H as [H | [H | H]]; subst; try by (rewrite /In; propositional).
+      right; right; by rewrite rotate_right_In_iff.
+    Qed.
+
+    (* this is awful, we should really be using proof search instead *)
+    Ltac solve_In :=
+      match goal with
+      | [ H : In _ (Node _ _ _) |- _ ] => destruct H; simplify; subst; eauto
+      | [ H : _ ∨ _ |- _] => destruct H; subst; eauto
+      | [ H : In _ (rotate_left _ _ _) |- _ ] => rewrite rotate_left_In_iff in H
+      | [ H : In _ (rotate_right _ _ _) |- _ ] => rewrite rotate_right_In_iff in H
+      | [ |- In _ (rotate_left _ _ _) ] => rewrite rotate_left_In_iff
+      | [ |- In _ (rotate_right _ _ _) ] => rewrite rotate_right_In_iff
+      | [ |- In ?x (Node ?x _ _) ] => rewrite /In; propositional
+      | [ _ : In ?x ?t |- In ?x (Node _ ?t _) ] => rewrite /In; propositional
+      | [ _ : In ?x ?t |- In ?x (Node _ _ ?t) ] => rewrite /In; propositional
+      | [ |- In _ (Node _ (rotate_left _ _ _) _) ] => apply rotate_left_In_tac1
+      | [ |- In _ (Node _ _ (rotate_left _ _ _)) ] => apply rotate_left_In_tac2
+      | [ |- In _ (Node _ (rotate_right _ _ _) _) ] => apply rotate_right_In_tac1
+      | [ |- In _ (Node _ _ (rotate_right _ _ _)) ] => apply rotate_right_In_tac2
+      end.
+
+    Lemma balance_left_In_complete x v l r : In x (Node v l r) → In x (balance_left v l r).
+    Proof.
+      functional induction (balance_left v l r); simplify; repeat solve_In.
+    Qed.
+
+    Lemma balance_right_In_complete x v l r : In x (Node v l r) → In x (balance_right v l r).
+    Proof.
+      functional induction (balance_right v l r); simplify; repeat solve_In.
+    Qed.
+
+    Lemma balance_left_In_correct x v l r : In x (balance_left v l r) → In x (Node v l r).
+    Proof.
+      functional induction (balance_left v l r); simplify; tauto || (repeat solve_In).
+    Qed.
+
+    Lemma balance_right_In_correct x v l r : In x (balance_right v l r) → In x (Node v l r).
+    Proof.
+      functional induction (balance_right v l r); simplify; tauto || (repeat solve_In).
+    Qed.
+
+    Lemma balance_left_In_iff x v l r : In x (balance_left v l r) <-> In x (Node v l r).
+    Proof.
+      split; by eauto using balance_left_In_correct, balance_left_In_complete.
+    Qed.
+
+    Lemma balance_right_In_iff x v l r : In x (balance_right v l r) <-> In x (Node v l r).
+    Proof.
+      split; by eauto using balance_right_In_correct, balance_right_In_complete.
+    Qed.
+
+    Hint Extern 1 (In _ (balance_left _ _ _)) => apply balance_left_In_complete : core.
+    Hint Extern 1 (In _ (balance_right _ _ _)) => apply balance_right_In_complete : core.
+    Hint Rewrite balance_left_In_iff balance_right_In_iff : core.
+
+    (* INSERT IS CORRECT WRT TO IN *)
+    Theorem insert_In_complete1 x y t : In x t → In x (insert y t).
+    Proof.
+      move => hyp.
+      functional induction (insert y t); simplify; try by eauto; repeat solve_In.
+    Qed.
+
+    Theorem insert_In_complete2 x t : In x (insert x t).
+    Proof.
+      functional induction (insert x t); simplify; by eauto.
+    Qed.
+
+    Theorem insert_In_correct x y t : In x (insert y t) → x = y ∨ In x t.
+    Proof.
+      functional induction (insert y t); simplify; eauto; repeat solve_In.
+    - apply IHt0 in H; by repeat solve_In.
+    - apply IHt0 in H; by repeat solve_In.
+    Qed.
+
+    (* note, insert is only idempotent if it is already balanced *)
+
+    Lemma invert_Balanced_left v l r : Balanced (Node v l r) → Balanced l.
+    Proof.
+      move=>H; by invert H.
+    Qed.
+
+    Lemma invert_Balanced_right v l r : Balanced (Node v l r) → Balanced r.
+    Proof.
+      move=>H; by invert H.
+    Qed.
+
+    Lemma rotate_left_height_le v l r :
+      height (rotate_left v l r) ≤ 1 + height (Node v l r).
+    Proof.
+      destruct r; by crush.
+    Qed.
+
+    Lemma rotate_right_height_le v l r :
+      height (rotate_right v l r) ≤ 1 + height (Node v l r).
+    Proof.
+      destruct l; by crush.
+    Qed.
+
+    Lemma rotate_left_height_ge v l r :
+      l ≠ Nil →
+      height (Node v l r) ≤ 1 + height (rotate_left v l r).
+    Proof.
+      destruct r; by crush.
+    Qed.
+
+    Lemma rotate_right_height_ge v l r :
+      r ≠ Nil →
+      height (Node v l r) ≤ 1 + height (rotate_right v l r).
+    Proof.
+      destruct l; by crush.
+    Qed.
+
+    Lemma rotate_left_height_change v l r :
+      (height (rotate_left v l r) = height (Node v l r))
+      ∨ (height (rotate_left v l r) = 1 + height (Node v l r))
+      ∨ (1 + height (rotate_left v l r) = height (Node v l r)).
+    Proof.
+      destruct r; by crush.
+    Qed.
+
+    Lemma rotate_right_height_change v l r :
+      (height (rotate_right v l r) = height (Node v l r))
+      ∨ (height (rotate_right v l r) = 1 + height (Node v l r))
+      ∨ (1 + height (rotate_right v l r) = height (Node v l r)).
+    Proof.
+      destruct l; by crush.
+    Qed.
+
+    Lemma rotate_left_right_heavy v l r :
+      (height l < height r)%nat → height (rotate_left v l r) ≤ height (Node v l r).
+    Proof.
+      destruct r; by crush.
+    Qed.
+
+    Lemma rotate_right_left_heavy v l r :
+      (height r < height l)%nat → height (rotate_right v l r) ≤ height (Node v l r).
+    Proof.
+      destruct l; by crush.
+    Qed.
+
+    Lemma rotate_left_right_heavy' v l r :
+      (height l < height r)%nat →
+        height (rotate_left v l r) = height (Node v l r)
+        ∨ 1 + height (rotate_left v l r) = height (Node v l r).
+    Proof.
+      destruct r; by crush.
+    Qed.
+
+    Lemma rotate_right_left_heavy' v l r :
+      (height r < height l)%nat →
+        height (rotate_right v l r) = height (Node v l r)
+        ∨ 1 + height (rotate_right v l r) = height (Node v l r).
+    Proof.
+      destruct l; by crush.
+    Qed.
+
+    Lemma rotate_left_right_heavy_1 v l rv rl rr :
+      (1 + height l < height (Node rv rl rr))%nat →
+      (height rl < height rr)%nat →
+      1 + height (rotate_left v l (Node rv rl rr)) = height (Node v l (Node rv rl rr)).
+    Proof.
+      by crush.
+    Qed.
+
+
+    Lemma rotate_left_equal v l r :
+      r ≠ Nil → height l = height r → height (rotate_left v l r) = 1 + height (Node v l r).
+    Proof.
+      destruct r; by crush.
+    Qed.
+
+    Lemma rotate_right_equal v l r :
+      l ≠ Nil → height l = height r → height (rotate_right v l r) = 1 + height (Node v l r).
+    Proof.
+      destruct l; by crush.
+    Qed.
+
+    Lemma balance_left_preserves_Balanced v l r : Balanced (Node v l r) → Balanced (balance_left v l r).
+    Proof.
+      move => Hbal.
+      functional induction (balance_left v l r); simplify; eauto.
+      - invert Hbal; by crush.
+      - invert Hbal; by crush.
+    Qed.
+
+    Lemma balance_right_preserves_Balanced v l r : Balanced (Node v l r) → Balanced (balance_right v l r).
+    Proof.
+      move => Hbal.
+      functional induction (balance_right v l r); simplify; eauto; invert Hbal; by crush.
+    Qed.
+
+    Lemma balance_left_Balanced_same v l r : Balanced (Node v l r) → balance_left v l r = Node v l r.
+    Proof.
+      move=> Hbal.
+      functional induction (balance_left v l r); simplify; eauto; invert Hbal; by crush.
+    Qed.
+
+    Lemma balance_right_Balanced_same v l r : Balanced (Node v l r) → balance_right v l r = Node v l r.
+    Proof.
+      move=>Hbal.
+      functional induction (balance_right v l r); simplify; eauto; invert Hbal; by crush.
+    Qed.
+
+    Lemma rotate_left_not_Nil v l r : rotate_left v l r = Nil → False.
+    Proof.
+      by destruct r.
+    Qed.
+
+    Lemma rotate_right_not_Nil v l r : rotate_right v l r = Nil → False.
+    Proof.
+      by destruct l.
+    Qed.
+    (* Hint Resolve rotate_left_not_Nil rotate_right_not_Nil : core. *)
+
+    Ltac rotate_not_nil :=
+      match goal with
+      | [ H : Node _ _ _ = Nil |- _ ] => by invert H
+      | [ H : rotate_left _ _ _ = Nil |- _ ] => exfalso; exact: rotate_left_not_Nil _ _ _ H
+      | [ H : rotate_right _ _ _ = Nil |- _ ] => exfalso; exact: rotate_right_not_Nil _ _ _ H
+      end.
+    Hint Extern 0 => rotate_not_nil : core.
+
+    Lemma balance_left_not_Nil v l r : balance_left v l r = Nil → False.
+    Proof.
+      rewrite /balance_left.
+      split_ifs; destruct l; try split_ifs; by crush.
+    Qed.
+
+    Lemma balance_right_not_Nil v l r : balance_right v l r = Nil → False.
+    Proof.
+      rewrite /balance_right.
+      split_ifs; destruct r; try split_ifs; by crush.
+    Qed.
+
+    Ltac balance_not_nil :=
+      match goal with
+      | [ H : balance_left _ _ _ = Nil |- _ ] => exfalso; exact: balance_left_not_Nil _ _ _ H
+      | [ H : balance_right _ _ _  = Nil |- _ ] => exfalso; exact: balance_right_not_Nil _ _ _ H
+      end.
+    Hint Extern 0 => balance_not_nil : core.
+
+    Lemma insert_not_Nil x t : insert x t ≠ Nil.
+    Proof.
+      move=>bad.
+      induction t.
+      - invert bad.
+      - rewrite /insert in bad.
+        elim_compare v x; rewrite -/insert in bad; by crush.
+    Qed.
+
+    Hint Extern 0 =>
+      match goal with
+      | [ H : insert _ _ = Nil |- _ ] => exfalso; exact: insert_not_Nil _ _ H
+      end : core.
+
+    Ltac gen_destruct exp :=
+      let eq := fresh "Heq" in
+      let e := fresh "e" in
+      move eq : exp => e;
+      destruct e.
+
+    Lemma balance_left_height_le v l r :
+      height (balance_left v l r) ≤ height (Node v l r).
+    Proof.
+      functional induction (balance_left v l r); simplify; eauto; crush.
+      destruct lr; by crush.
+    Qed.
+
+    Lemma balance_right_height_le v l r :
+      height (balance_right v l r) ≤ height (Node v l r).
+    Proof.
+      functional induction (balance_right v l r); simplify; eauto; crush.
+      destruct rl; by crush.
+    Qed.
+
+    Lemma balance_left_height_ge v l r :
+      height (Node v l r) ≤ 2 + height (balance_left v l r).
+    Proof.
+      functional induction (balance_left v l r).
+      - by crush.
+      - by crush.
+      - repeat ltb_to_lt.
+        destruct (rotate_left_height_change lv ll lr) as [|[|]],
+            (rotate_right_height_change v (rotate_left lv ll lr) r) as [|[|]]; by crush.
+      - ltb_to_lt.
+        by crush.
+    Qed.
+
+    Lemma balance_right_height_ge v l r :
+      height (Node v l r) ≤ 2 + height (balance_right v l r).
+    Proof.
+      functional induction (balance_right v l r).
+      - by crush.
+      - by crush.
+      - destruct (rotate_right_height_change rv rl rr) as [|[|]],
+            (rotate_left_height_change v l (rotate_right rv rl rr)) as [|[|]]; by crush.
+      - by crush.
+    Qed.
+
+    Hint Extern 0 =>
+      match goal with
+      | [ H : (?a < ?b)%nat |- context[Nat.max ?a ?b] ] =>
+          rewrite (Nat.max_r _ _ (Nat.lt_le_incl _ _ H))
+      | [ H : (?b < ?a)%nat |- context[Nat.max ?a ?b] ] =>
+          rewrite (Nat.max_l _ _ (Nat.lt_le_incl _ _ H))
+      end : core.
+
+
+    Lemma insert_height_upper_bound x t : height (insert x t) ≤ 1 + height t.
+    Proof.
+      functional induction (insert x t); [by crush| lia | | ].
+      - transitivity (height (Node v l (insert x r))); [apply balance_right_height_le|].
+        rewrite /height -/height.
+        lia.
+      - transitivity (height (Node v (insert x l) r)); [apply balance_left_height_le|].
+        rewrite /height -/height; lia.
+    Qed.
+
+    Lemma eq_or_succ_cases {a b} : a ≤ b → b ≤ 1 + a → b = a ∨ b = 1 + a.
+    Proof.
+      lia.
+    Qed.
+
+    Ltac linear_arithmetic' := intros;
+      repeat match goal with
+      | [ |- S _ ≤ S _ ] =>
+          apply le_n_S
+      | [ H : (S _ < S _)%nat |- _ ] => rewrite -Nat.succ_lt_mono in H
+      | [ H : S _ = S _ |- _ ] => apply Nat.succ_inj in H
+      | [ |- context[Nat.max ?a ?b] ] =>
+        let Heq := fresh "Heq" in destruct (Nat.max_spec a b) as [[? Heq] | [? Heq]];
+          rewrite -> Heq in *; clear Heq
+      | [ _ : context[Nat.max ?a ?b] |- _ ] =>
+        let Heq := fresh "Heq" in destruct (Nat.max_spec a b) as [[? Heq] | [? Heq]];
+          rewrite -> Heq in *; clear Heq
+      | [ |- context[min ?a ?b] ] =>
+        let Heq := fresh "Heq" in destruct (Nat.min_spec a b) as [[? Heq] | [? Heq]];
+          rewrite -> Heq in *; clear Heq
+      | [ _ : context[min ?a ?b] |- _ ] =>
+        let Heq := fresh "Heq" in destruct (Nat.min_spec a b) as [[? Heq] | [? Heq]];
+          rewrite -> Heq in *; clear Heq
+      end.
+
+    Lemma invert_insert x t : ∃ v l r, insert x t = Node v l r.
+    Proof.
+      functional induction (insert x t); eauto.
+      - destruct IHt0 as [v' [l' [r' Heq]]].
+        rewrite {}Heq.
+        functional induction (balance_right v l (Node v' l' r')); eauto.
+        + destruct rl; simplify; eauto.
+        + destruct rl; simplify; eauto.
+      - destruct IHt0 as [v' [l' [r' Heq]]].
+        rewrite {}Heq.
+        functional induction (balance_left v (Node v' l' r') r); eauto;
+        destruct lr; simplify; eauto.
+    Qed.
+
+    (* this is in general, NOT TRUE!! *)
+    Lemma hmmm v l r :
+      Balanced l → Balanced r → 2 + height l = height r →
+      Balanced (balance_right v l r).
+    Proof.
+    Abort.
+    (* AVL trees work specifically because you can only ever have at most 1 broken invariant, not 2 *)
+
+    Definition left_child t :=
+      match t with
+      | Nil => Nil
+      | Node _ l _ => l
+      end.
+
+    Definition right_child t :=
+      match t with
+      | Nil => Nil
+      | Node _ _ r => r
+      end.
+
+    Hint Unfold left_child right_child : core.
+    Lemma insert_preserves_Balanced0 x t :
+      Balanced t →
+      Balanced (insert x t) ∧
+        height t ≤ height (insert x t) ∧
+        (t ≠ Nil →
+         1 + height t = height (insert x t) →
+         height (left_child (insert x t)) ≠ height (right_child (insert x t))).
+    Proof.
+      functional induction (insert x t); move => t_bal; repeat split; simplify; eauto.
+      - exfalso; lia.
+      - have r_bal : Balanced r by invert t_bal.
+        have {r_bal}IHt0 := IHt0 r_bal.
+        destruct IHt0 as [insert_bal [IH_height IH_unbal]].
+        have r_height_lower := insert_height_upper_bound x r.
+        invert t_bal; simplify.
+        + (* equal heights *)
+          apply balance_right_preserves_Balanced.
+          destruct (eq_or_succ_cases IH_height r_height_lower) as [H|H].
+          * apply Balanced_equal; by crush.
+          * apply Balanced_right_heavy; by crush.
+        + (* left heavy *)
+          apply balance_right_preserves_Balanced.
+          destruct (eq_or_succ_cases IH_height r_height_lower).
+          * apply Balanced_left_heavy; by crush.
+          * apply Balanced_equal; by crush.
+        + (* right heavy *)
+          destruct (eq_or_succ_cases IH_height r_height_lower) as [H|H];
+            [apply balance_right_preserves_Balanced, Balanced_right_heavy; by crush|].
+          (* now we have a +2 height diff, so balance_right must kick in. *)
+          destruct r; [crush|].
+          have r_nonnil : Node v0 r1 r2 ≠ Nil by done.
+          symmetry in H.
+          have {r_nonnil}IH_unbal := IH_unbal r_nonnil H.
+          functional induction (balance_right v l (insert x (Node v0 r1 r2))); simplify; eauto; try lia.
+          * invert insert_bal; try lia.
+            linear_arithmetic'; invert H3; try lia; apply Balanced_equal; crush.
+          * have {e2 IH_unbal} IH_unbal : 1 + height rr = height rl by (invert insert_bal; lia).
+            destruct rl; [simplify; lia|].
+            simplify.
+            invert insert_bal; invert H3; linear_arithmetic'; simplify; try lia;
+              invert H6; try lia; apply Balanced_equal; crush.
+      - have r_bal : Balanced r by invert t_bal.
+        have {r_bal IHt0}[insert_bal [height_le unbal]] := IHt0 r_bal.
+        have r_height_lower := insert_height_upper_bound x r.
+        destruct r.
+        { invert t_bal; simplify; try lia.
+          rewrite (height_eq_zero_nil l H4); simplify; crush.
+          destruct l; [simplify; lia|simplify].
+          have l1_nil : height l1 = 0 by lia.
+          have l2_nil : height l2 = 0 by lia.
+          rewrite (height_eq_zero_nil l1 l1_nil) (height_eq_zero_nil l2 l2_nil); simplify; crush.
+        }
+        have {}unbal := unbal node_neq_nil.
+        destruct (eq_or_succ_cases height_le r_height_lower) as [H|H].
+        {
+          functional induction (balance_right v l (insert x (Node v0 r1 r2)));
+            invert t_bal;
+            simplify; try lia.
+        }
+        functional induction (balance_right v l (insert x (Node v0 r1 r2))); invert t_bal; simplify; try lia.
+        destruct rl; [simplify; lia|].
+        invert insert_bal; simplify; try lia.
+      - have r_bal : Balanced r by invert t_bal.
+        have {r_bal IHt0}[insert_bal [height_ge unbal]] := IHt0 r_bal.
+        have r_height_lower := insert_height_upper_bound x r.
+        destruct r.
+        {
+          clear unbal height_ge insert_bal H r_height_lower.
+          simplify.
+          invert t_bal; [| |simplify; try lia].
+          -
+            rewrite (height_eq_zero_nil l H5) /balance_right; simplify; lia.
+          - exfalso.
+            rewrite /balance_right in H0; simplify; lia.
+        }
+        have l_bal_diff : (1 + height l < height (balance_right v l (insert x (Node v0 r1 r2))))%nat by lia.
+        functional induction (balance_right v l (insert x (Node v0 r1 r2))); simplify; try lia.
+        destruct rl; [simplify; lia|].
+        invert insert_bal; simplify; lia.
+      - (* all cases from here on are symmetric. *)
+        have l_bal : Balanced l by invert t_bal.
+        have {l_bal}IHt0 := IHt0 l_bal.
+        destruct IHt0 as [insert_bal [IH_height IH_unbal]].
+        have l_height_lower := insert_height_upper_bound x l.
+        invert t_bal; simplify.
+        + (* equal heights *)
+          apply balance_left_preserves_Balanced.
+          destruct (eq_or_succ_cases IH_height l_height_lower) as [H|H].
+          * apply Balanced_equal; by crush.
+          * apply Balanced_left_heavy; by crush.
+        + (* left heavy *)
+          destruct (eq_or_succ_cases IH_height l_height_lower) as [H|H];
+            [apply balance_left_preserves_Balanced, Balanced_left_heavy; by crush|].
+          (* now we have a +2 height diff, so balance_left must kick in *)
+          destruct l; [crush|].
+          symmetry in H.
+          have {}IH_unbal := IH_unbal node_neq_nil H.
+          functional induction (balance_left v (insert x (Node v0 l1 l2)) r); simplify; eauto; try lia.
+          * invert insert_bal; try lia.
+            linear_arithmetic'; invert H2; try lia; apply Balanced_equal; crush.
+          * have {e2 IH_unbal}IH_unbal : 1 + height ll = height lr by (invert insert_bal; lia).
+            destruct lr; [simplify; lia|].
+            invert insert_bal; invert H2; invert H7; simplify; try lia; apply Balanced_equal; crush.
+        + (* right heavy *)
+          apply balance_left_preserves_Balanced.
+          destruct (eq_or_succ_cases IH_height l_height_lower).
+          * apply Balanced_right_heavy; by crush.
+          * apply Balanced_equal; by crush.
+      - have l_bal : Balanced l by invert t_bal.
+        have {l_bal}IHt0 := IHt0 l_bal.
+        have l_height_lower := insert_height_upper_bound x l.
+        destruct IHt0 as [insert_bal [insert_height_ge unbal]].
+        destruct l.
+        {
+          invert t_bal; simplify; try lia.
+          symmetry in H4.
+          rewrite (height_eq_zero_nil r H4); simplify; crush.
+          destruct r; [simplify; lia| simplify].
+          have r1_nil : height r1 = 0 by lia.
+          have r2_nil : height r2 = 0 by lia.
+          rewrite (height_eq_zero_nil _ r1_nil) (height_eq_zero_nil _ r2_nil); simplify; crush.
+        }
+        have {}unbal := unbal node_neq_nil.
+        destruct (eq_or_succ_cases insert_height_ge l_height_lower) as [H|H].
+        {
+          functional induction (balance_left v (insert x (Node v0 l1 l2)) r);
+            invert t_bal; simplify; lia.
+        }
+        functional induction (balance_left v (insert x (Node v0 l1 l2)) r); invert t_bal; simplify; try lia.
+        destruct lr; [simplify; lia|].
+        invert insert_bal; simplify; lia.
+      - have l_bal : Balanced l by invert t_bal.
+        have {l_bal IHt0}[insert_bal [insert_height_ge unbal]] := IHt0 l_bal.
+        have l_height_lower := insert_height_upper_bound x l.
+        destruct l.
+        {
+          clear unbal insert_height_ge insert_bal H.
+          simplify.
+          invert t_bal; [| simplify; try lia|].
+          - symmetry in H5.
+            rewrite (height_eq_zero_nil r H5) /balance_left; simplify; lia.
+          - exfalso.
+            rewrite /balance_left in H0; simplify; lia.
+        }
+        have r_bal_diff : (1 + height r < height (balance_left v (insert x (Node v0 l1 l2)) r))%nat by lia.
+        functional induction (balance_left v (insert x (Node v0 l1 l2)) r); simplify; try lia.
+        destruct lr; [simplify; lia|].
+        invert insert_bal; simplify; lia.
+    Qed.
+
+
+    (* INSERT PRESERVES BALANCE! *)
+    Theorem insert_preserves_Balanced x t : Balanced t → Balanced (insert x t).
+    Proof.
+      move => t_bal.
+      have := insert_preserves_Balanced0 x t_bal.
+      tauto.
+    Qed.
+
+    Lemma insert_height_lower_bound x t : Balanced t → height t ≤ height (insert x t).
+      move => t_bal.
+      have := insert_preserves_Balanced0 x t_bal; tauto.
+    Qed.
+
+End AVL.
