README.md
@@ -1,0 +1,19 @@
+# README
+
+All work is done with Rocq v8.20.
+
+The filestructure is as follows:
+- `AVL.v` contains most of the work.
+- `Util.v` contains a few utilities -- why something is in `AVL.v` instead of `Util.v` is usually just sloppiness.
+- `AVLHeightFacts.v` contains the development of logarithmic height for AVL trees.
+- `AVLResults.v` contains all the key results.
+- `AVL_incorrect.v` contains an older version of `AVL.v`, developed with incorrect rebalancing functions. It culminates in a proof that insertion still preserves AVL balance despite the incorrect definition.
+- `avl.cc` an implementation of AVL trees, based on the implementation in `AVL.v`, which correctly solves the problem `ds4` on the online judge DMOJ (https://dmoj.ca/problem/ds4). See this submission: https://dmoj.ca/submission/7120643
+
+# COMPILATION
+
+Just run `make`.
+
+Note that this process takes 70s on my Ryzen 5 5600X, so expect it to take a while.
+On another classmate's laptop, it took an entire 5 minutes.
+
